fstar/new/MLS.TreeSyncTreeKEMBinder.fst
@@ -33,6 +33,30 @@ let encrypted_path_secret_nt_to_tk (cs:ciphersuite) (x:hpke_ciphertext_nt): resu
       TK.ciphertext = x.hcn_ciphertext;
     })
 
+val treesync_to_treekem_node_package: cs:ciphersuite -> nat -> TS.node_package_t -> result (TK.key_package cs)
+let treesync_to_treekem_node_package cs nb_left_leaves np =
+  content <-- from_option "treesync_to_treekem_node_package: Couldn't parse node content"
+    ((ps_to_pse ps_node_package_content).parse_exact (pub_to_secret np.TS.np_content));
+  path_secret_ciphertext <-- mapM (encrypted_path_secret_nt_to_tk cs) (Seq.seq_to_list content.npc_encrypted_path_secret);
+  unmerged_leaves <-- mapM (fun (unmerged_leaf:nat) ->
+    if not (nb_left_leaves <= unmerged_leaf) then
+      error "treesync_to_treekem_node_package: unmerged_leaf index too small"
+    else
+      return ((unmerged_leaf - nb_left_leaves) <: nat)
+  ) np.TS.np_unmerged_leafs;
+  if not (Seq.length content.npc_public_key = hpke_public_key_length cs) then
+    error "treesync_to_treekem_node_package: public key has wrong length"
+  else (
+    return ({
+      TK.kp_public_key = content.npc_public_key;
+      TK.kp_version = np.TS.np_version;
+      TK.kp_last_group_context = content.npc_last_group_context;
+      TK.kp_unmerged_leafs = unmerged_leaves;
+      TK.kp_path_secret_from = (np.TS.np_content_dir);
+      TK.kp_path_secret_ciphertext = path_secret_ciphertext;
+    })
+  )
+
 val treesync_to_treekem_aux: #l:nat -> #n:tree_size l -> cs:ciphersuite -> nat -> TS.treesync l n -> result (TK.treekem cs l n)
 let rec treesync_to_treekem_aux #l #n cs nb_left_leaves t =
   match t with
@@ -55,28 +79,8 @@ let rec treesync_to_treekem_aux #l #n cs nb_left_leaves t =
     | None ->
       return (TNode None tk_left tk_right)
     | Some np ->
-      content <-- from_option "treesync_to_treekem: Couldn't parse node content"
-        ((ps_to_pse ps_node_package_content).parse_exact (pub_to_secret np.TS.np_content));
-      path_secret_ciphertext <-- mapM (encrypted_path_secret_nt_to_tk cs) (Seq.seq_to_list content.npc_encrypted_path_secret);
-      unmerged_leaves <-- mapM (fun (unmerged_leaf:nat) ->
-        if not (nb_left_leaves <= unmerged_leaf) then
-          error "treesync_to_treekem: unmerged_leaf index too small"
-        else
-          return ((unmerged_leaf - nb_left_leaves) <: nat)
-      ) np.TS.np_unmerged_leafs;
-      if not (Seq.length content.npc_public_key = hpke_public_key_length cs) then
-        error "treesync_to_treekem: public key has wrong length"
-      else (
-        let kp: TK.key_package cs = {
-          TK.kp_public_key = content.npc_public_key;
-          TK.kp_version = np.TS.np_version;
-          TK.kp_last_group_context = content.npc_last_group_context;
-          TK.kp_unmerged_leafs = unmerged_leaves;
-          TK.kp_path_secret_from = (np.TS.np_content_dir);
-          TK.kp_path_secret_ciphertext = path_secret_ciphertext;
-        } in
-        return (TNode (Some kp) tk_left tk_right)
-      )
+      kp <-- treesync_to_treekem_node_package cs nb_left_leaves np;
+      return (TNode (Some kp) tk_left tk_right)
   end
 
 val treesync_to_treekem: #l:nat -> #n:tree_size l -> cs:ciphersuite -> TS.treesync l n -> result (TK.treekem cs l n)
@@ -94,12 +98,34 @@ let encrypted_path_secret_tk_to_nt (#cs:ciphersuite) (x:TK.path_secret_ciphertex
       hcn_ciphertext = x.TK.ciphertext;
     })
 
-#push-options "--z3rlimit 50"
-val treekem_to_treesync_aux: #l:nat -> #n:tree_size l -> #i:leaf_index n -> #cs:ciphersuite -> nat -> TS.leaf_package_t -> TK.pathkem cs l n i -> TK.path_parent_hash l n i -> result (TS.pathsync l n i)
-let rec treekem_to_treesync_aux #l #n #i #cs nb_left_leaves old_leaf_package pk pph =
-  match pk, pph with
-  | PLeaf mi, PLeaf parent_hash ->
-    return (PLeaf (Some ({
+val treekem_to_treesync_node_package: #cs:ciphersuite -> nat -> TK.key_package cs -> result TS.external_node_package_t
+let treekem_to_treesync_node_package #cs nb_left_leaves kp =
+  ciphertexts <-- mapM encrypted_path_secret_tk_to_nt kp.TK.kp_path_secret_ciphertext;
+  if not (byte_length ps_hpke_ciphertext ciphertexts < pow2 16) then
+    internal_failure "treekem_to_treesync: ciphertexts too long"
+  else if not (Seq.length kp.TK.kp_last_group_context < pow2 64) then
+    internal_failure "treekem_to_treesync: last group context too long (internal error)"
+  else begin
+    Seq.lemma_list_seq_bij ciphertexts;
+    let np_content = ps_node_package_content.serialize ({
+      npc_public_key = kp.TK.kp_public_key;
+      npc_encrypted_path_secret = Seq.seq_of_list ciphertexts;
+      npc_last_group_context = kp.TK.kp_last_group_context;
+    }) in
+    return ({
+      TS.np_version = kp.TK.kp_version;
+      TS.np_content_dir = kp.TK.kp_path_secret_from;
+      TS.np_unmerged_leafs = List.Tot.map (fun (x:nat) -> (x + nb_left_leaves <: nat)) kp.TK.kp_unmerged_leafs;
+      TS.np_parent_hash = Seq.empty;
+      TS.np_content = secret_to_pub np_content;
+    } <: TS.external_node_package_t)
+  end
+
+val treekem_to_treesync_aux: #l:nat -> #n:tree_size l -> #i:leaf_index n -> #cs:ciphersuite -> nat -> TS.leaf_package_t -> TK.pathkem cs l n i -> result (TS.external_pathsync l n i)
+let rec treekem_to_treesync_aux #l #n #i #cs nb_left_leaves old_leaf_package pk =
+  match pk with
+  | PLeaf mi ->
+    return (PLeaf ({
       TS.lp_credential = old_leaf_package.TS.lp_credential;
       TS.lp_version = mi.TK.mi_version;
       TS.lp_content = secret_to_pub (ps_leaf_package_content.serialize ({
@@ -107,38 +133,18 @@ let rec treekem_to_treesync_aux #l #n #i #cs nb_left_leaves old_leaf_package pk 
       }));
       TS.lp_extensions = old_leaf_package.TS.lp_extensions; //TODO probably the parent hash should change?
       TS.lp_signature = old_leaf_package.TS.lp_signature; //TODO the signature definitely has to change
-    })))
-  | PSkip _ pk', PSkip _ pph' ->
-    result <-- treekem_to_treesync_aux nb_left_leaves old_leaf_package pk' pph';
+    }))
+  | PSkip _ pk' ->
+    result <-- treekem_to_treesync_aux nb_left_leaves old_leaf_package pk';
     return (PSkip _ result)
-  | PNode kp pk_next, PNode parent_hash pph_next ->
+  | PNode kp pk_next ->
     let (|dir, _|) = child_index l i in
     let new_left_leaves = (if dir = Left then nb_left_leaves else nb_left_leaves + pow2 (l-1)) in
-    next <-- treekem_to_treesync_aux new_left_leaves old_leaf_package pk_next pph_next;
-    ciphertexts <-- mapM encrypted_path_secret_tk_to_nt kp.TK.kp_path_secret_ciphertext;
-    if not (byte_length ps_hpke_ciphertext ciphertexts < pow2 16) then
-      internal_failure "treekem_to_treesync: ciphertexts too long"
-    else if not (Seq.length kp.TK.kp_last_group_context < pow2 64) then
-      internal_failure "treekem_to_treesync: last group context too long (internal error)"
-    else begin
-      Seq.lemma_list_seq_bij ciphertexts;
-      let np_content = ps_node_package_content.serialize ({
-        npc_public_key = kp.TK.kp_public_key;
-        npc_encrypted_path_secret = Seq.seq_of_list ciphertexts;
-        npc_last_group_context = kp.TK.kp_last_group_context;
-      }) in
-      let np = ({
-        TS.np_version = kp.TK.kp_version;
-        TS.np_content_dir = kp.TK.kp_path_secret_from;
-        TS.np_unmerged_leafs = List.Tot.map (fun (x:nat) -> (x + nb_left_leaves <: nat)) kp.TK.kp_unmerged_leafs;
-        TS.np_parent_hash = parent_hash;
-        TS.np_content = secret_to_pub np_content;
-      }) in
-      return (PNode (Some np) next)
-    end
-#pop-options
+    next <-- treekem_to_treesync_aux new_left_leaves old_leaf_package pk_next;
+    np <-- treekem_to_treesync_node_package nb_left_leaves kp;
+    return (PNode np next)
 
-val treekem_to_treesync: #l:nat -> #n:tree_size l -> #i:leaf_index n -> #cs:ciphersuite -> TS.leaf_package_t -> TK.pathkem cs l n i -> TK.path_parent_hash l n i -> result (TS.pathsync l n i)
-let treekem_to_treesync #l #n #i #cs old_leaf_package pk pph =
-  treekem_to_treesync_aux 0 old_leaf_package pk pph
+val treekem_to_treesync: #l:nat -> #n:tree_size l -> #i:leaf_index n -> #cs:ciphersuite -> TS.leaf_package_t -> TK.pathkem cs l n i -> result (TS.external_pathsync l n i)
+let treekem_to_treesync #l #n #i #cs old_leaf_package pk =
+  treekem_to_treesync_aux 0 old_leaf_package pk
 
