fstar/new/MLS.TreeSync.ParentHash.fst
@@ -1,0 +1,119 @@
+module MLS.TreeSync.ParentHash
+
+open Lib.ByteSequence
+open MLS.TreeSync.Types
+open MLS.TreeKEM.Types
+open MLS.TreeKEM
+open MLS.TreeSyncTreeKEMBinder
+open MLS.Crypto
+open MLS.Tree
+open MLS.NetworkTypes
+open MLS.Parser
+open MLS.Result
+
+#set-options "--ifuel 1 --fuel 1"
+
+noeq type parent_hash_input_nt = {
+  phin_public_key: hpke_public_key_nt;
+  phin_parent_hash: blbytes ({min=0;max=255});
+  phin_original_child_resolution: blseq hpke_public_key_nt ps_hpke_public_key ({min=0; max=(pow2 32)-1});
+}
+
+val ps_parent_hash_input: parser_serializer parent_hash_input_nt
+let ps_parent_hash_input =
+  let open MLS.Parser in
+  isomorphism parent_hash_input_nt
+    (
+      _ <-- ps_hpke_public_key;
+      _ <-- ps_bytes _;
+      ps_seq _ ps_hpke_public_key
+    )
+  (fun (|public_key, (|parent_hash, original_child_resolution|)|) -> {
+    phin_public_key = public_key;
+    phin_parent_hash = parent_hash;
+    phin_original_child_resolution = original_child_resolution;
+  })
+  (fun x -> (|x.phin_public_key, (|x.phin_parent_hash, x.phin_original_child_resolution|)|))
+
+val compute_parent_hash_treekem: #cs:ciphersuite -> #l:nat -> #n:tree_size l -> hpke_public_key cs -> bytes -> treekem cs l n -> list (hpke_public_key cs) -> result (lbytes (hash_length cs))
+let compute_parent_hash_treekem #cs #l #n public_key parent_hash sibling forbidden_public_keys =
+  let sibling_resolution = tree_resolution sibling in
+  let original_child_resolution = List.Tot.filter (fun pk ->
+    //TODO: this should break secret independance?
+    not (List.Tot.mem pk forbidden_public_keys)
+  ) sibling_resolution in
+  let original_child_resolution_nt = List.Tot.map (fun (x:hpke_public_key cs) -> x <: hpke_public_key_nt) original_child_resolution in
+  if not (Seq.length parent_hash < 256) then
+    internal_failure "compute_parent_hash: parent_hash too long"
+  else if not (byte_length ps_hpke_public_key original_child_resolution_nt < pow2 32) then
+    internal_failure "compute_parent_hash: original_child_resolution too big"
+  else (
+    Seq.lemma_list_seq_bij original_child_resolution_nt;
+    hash_hash cs (ps_parent_hash_input.serialize ({
+      phin_public_key = public_key;
+      phin_parent_hash = parent_hash;
+      phin_original_child_resolution = Seq.seq_of_list original_child_resolution_nt;
+    }))
+  )
+
+//TODO possible performance optimisation: no need to convert root from treesync to treekem: we only need to convert its content
+val compute_parent_hash_from_sibling: #l:nat -> #ls:nat -> #n:tree_size l -> #ns:tree_size ls -> cs:ciphersuite -> hpke_public_key cs -> bytes -> nat -> treesync l n -> nat -> treesync ls ns -> result (lbytes (hash_length cs))
+let compute_parent_hash_from_sibling #l #ls #n #ns cs public_key parent_parent_hash nb_left_leaves_root root nb_left_leaves_sibling sibling =
+  root_kem <-- treesync_to_treekem_aux cs nb_left_leaves_root root;
+  sibling_kem <-- treesync_to_treekem_aux cs nb_left_leaves_sibling sibling;
+  root_kem_onp <-- (
+    match root_kem with
+    | TNode root_onp _ _ ->
+      return root_onp
+    | _ ->
+      internal_failure "compute_parent_hash_from_sibling: `root` must be an internal node"
+  );
+  let forbidden_keys =
+    match root_kem_onp with
+    | None -> []
+    | Some root_np ->
+      unmerged_leafs_resolution root_kem root_np.kp_unmerged_leafs
+  in
+  compute_parent_hash_treekem public_key parent_parent_hash sibling_kem forbidden_keys
+
+val compute_parent_hash_from_dir: #l:nat -> #n:tree_size l -> cs:ciphersuite -> hpke_public_key cs -> bytes -> nat -> treesync l n -> direction -> result (lbytes (hash_length cs))
+let compute_parent_hash_from_dir #l #n cs public_key parent_parent_hash nb_left_leaves root dir =
+  match root with
+  | TNode _ left right ->
+    let (_, sibling) = order_subtrees dir (left, right) in
+    let nb_left_leaves_sibling =
+      if dir = Left then
+        nb_left_leaves + (pow2 (l-1))
+      else
+        nb_left_leaves
+    in
+    compute_parent_hash_from_sibling cs public_key parent_parent_hash nb_left_leaves root nb_left_leaves_sibling sibling
+  | _ -> internal_failure "compute_parent_hash_from_dir: `root` must be an internal node"
+
+
+//TODO: this function has bad complexity (because some subtrees are converted a lot of time)
+//Do we care?
+val external_pathsync_to_pathsync_aux: #l:nat -> #n:tree_size l -> #i:leaf_index n -> cs:ciphersuite -> bytes -> nat -> treesync l n -> external_pathsync l n i -> result (pathsync l n i)
+let rec external_pathsync_to_pathsync_aux #l #n #i cs parent_parent_hash nb_left_leaves t p =
+  match t, p with
+  | _, PLeaf lp ->
+    //TODO check that the parent hash in lp is correct
+    return (PLeaf (Some lp))
+  | TSkip _ t', PSkip _ p' ->
+    result <-- external_pathsync_to_pathsync_aux cs parent_parent_hash nb_left_leaves t' p';
+    return (PSkip _ result)
+  | TNode _ left right, PNode np p_next ->
+    let (|dir, next_i|) = child_index l i in
+    let (child, sibling) = order_subtrees dir (left, right) in
+    let child_nb_left_leaves = if dir = Left then nb_left_leaves else nb_left_leaves + (pow2 (l-1)) in
+    public_key <-- (
+      kem_node_package <-- treesync_to_treekem_node_package cs nb_left_leaves np;
+      return kem_node_package.kp_public_key
+    );
+    parent_hash <-- compute_parent_hash_from_dir cs public_key parent_parent_hash nb_left_leaves t dir;
+    result_p_next <-- external_pathsync_to_pathsync_aux cs parent_hash child_nb_left_leaves child p_next;
+    return (PNode (Some ({np with np_parent_hash = parent_parent_hash;})) result_p_next)
+
+val external_pathsync_to_pathsync: #l:nat -> #n:tree_size l -> #i:leaf_index n -> cs:ciphersuite -> treesync l n -> external_pathsync l n i -> result (pathsync l n i)
+let external_pathsync_to_pathsync #l #n #i cs t p =
+  external_pathsync_to_pathsync_aux cs bytes_empty 0 t p
